smtlink/examples.lisp
@@ -1,0 +1,13 @@
+(add-include-book-dir :cp "/ubc/cs/home/y/yanpeng/project/ACL2/smtlink")
+(include-book "top" :dir :cp)
+(tshell-ensure)
+
+(defthm poly-ineq-example
+    (implies (and (rationalp x) (rationalp y)
+                  (<= (+ (* (/ 9 8) x x) (* y y)) 1)
+                      (<= (- (* x x) (* y y)) 1))
+	       (<= y (* 3 (- x (/ 17 8)) (- x (/ 17 8)))))
+    :hints(("Goal"
+      :clause-processor
+      (Smtlink clause nil state))))
+
